CertiGC/verif_Is_from.v
@@ -1,0 +1,174 @@
+Require Export compcert.common.Events.
+Require Export RamifyCoq.CertiGC.gc_spec.
+
+Definition valid_block (m : mem) (b : block) (o : ptrofs) (n : Z) : Prop :=
+  0 < n /\
+  Ptrofs.unsigned o + n <= Int.modulus /\
+  forall i : Z, 0 <= i < n ->
+                common.Memory.Mem.valid_pointer m b (Ptrofs.unsigned o + i) = true.
+
+Definition Is_from_sem : extcall_sem :=
+  fun _ args m1 trc ret m2 =>
+    m1 = m2 /\ trc = nil /\ 
+    match args with
+    | (Vptr b1 o1) :: (Vptr b2 o2) :: (Vptr b3 o3) :: nil =>
+      exists n : Z, 0 < n /\ Ptrofs.unsigned o1 + n < Int.modulus /\
+                    (b1 = b2) /\ (Ptrofs.unsigned o1 + n = Ptrofs.unsigned o2) /\
+                    valid_block m1 b1 o1 n /\
+                    common.Memory.Mem.valid_pointer m1 b3 (Ptrofs.unsigned o3) = true /\
+                    ((b1 = b3 /\ (Ptrofs.unsigned o1 <=
+                                  Ptrofs.unsigned o3 <
+                                  Ptrofs.unsigned o2)
+                      /\ ret = Vone) \/
+                     (((b1 <> b3) \/
+                       (b1 = b3 /\
+                        (Ptrofs.unsigned o3 < Ptrofs.unsigned o1 \/
+                         Ptrofs.unsigned o3 >= Ptrofs.unsigned o2)))
+                      /\ ret = Vzero))
+    | _ => False
+    end.
+
+Definition Is_from_sig : signature :=
+  mksignature (AST.Tint :: AST.Tint :: AST.Tint :: nil) (Some AST.Tint) cc_default.
+
+Lemma Is_from_extcall: extcall_properties Is_from_sem Is_from_sig.
+Proof.
+  constructor.
+  - intros. destruct H as [_ [_ ?]].
+    do 4 (destruct vargs; try destruct v; try contradiction).
+    destruct H as [_ [_ [_ [_ [_ [_ [_ ?]]]]]]].
+    destruct H as [[_ [_ ?]] | [_ ?]]; subst; apply I.
+  - intros. apply H0.
+  - intros. destruct H as [? _]. subst m1. apply H0.
+  - intros. destruct H as [? _]. subst m1. apply H1.
+  - intros. destruct H as [? _]. subst m1.
+    apply Mem.unchanged_on_refl.
+  - intros. exists vres, m1'.
+    destruct H as [? [? ?]]. subst m2 t.
+    split. 2: { split. apply Val.lessdef_refl. split. trivial. apply Mem.unchanged_on_refl. }
+    split. trivial. split. trivial.
+    do 4 (destruct vargs; try destruct v; try contradiction).    
+    inversion H1. inversion H4. inversion H6. inversion H11.
+    inversion H13. inversion H18. inversion H20. subst. clear H4 H11 H18 H20 H13 H6 H1.
+    destruct H3 as [n [? [? [? [? ?]]]]].
+    exists n. repeat (split; [assumption|]). clear H H1 H2 H3. 
+    destruct H4 as [? [? ?]].
+    split. {
+      clear -H H0.
+      destruct H as [? [? ?]]. do 2 (split; trivial).
+      intros i0 Hx. specialize (H2 i0 Hx).
+      eapply Mem.valid_pointer_extends; eauto. }
+    split. eapply Mem.valid_pointer_extends; eauto.
+    tauto.
+  - intros. exists f, vres, m1'. destruct H0 as [? [? ?]]. split.
+    2: {
+      split.
+      - do 4 (destruct vargs; try destruct v; try contradiction). inversion H2. inversion H7. inversion H9.
+      inversion H17. inversion H19.
+      inversion H27. inversion H29.
+      destruct H4 as [n [? [? [? [? [? [? ?]]]]]]]. 
+      destruct vres; auto.  
+      now destruct H41.
+      - repeat (split; [now subst|]).
+        apply mem_lemmas.inject_separated_same_meminj.
+    }
+    split3; trivial.
+    do 4 (destruct vargs; try destruct v; try contradiction).
+    inversion H2; inversion H7; inversion H9;
+      inversion H17; inversion H19; inversion H27;
+        inversion H29; subst.
+    clear H2 H7 H9 H17 H19 H27 H29.
+    destruct H4 as [n [? [? [? [? [? [? ?]]]]]]].
+    subst. exists n. rewrite H22 in H12; inversion H12.
+    split3; [| |split3; [| |split3]]; trivial.
+    5: { destruct H7.
+         - destruct H3 as [? [? ?]]; subst.
+           rewrite H32 in H22; inversion H22.
+           left; split3; trivial. admit.
+         - destruct H3; subst; destruct H3.
+           + right; split; trivial; left. admit.
+           + right; split; trivial. right. destruct H3; split.
+             subst. rewrite H32 in H22; now inversion H22.
+             destruct H7; [left|right].
+             * admit.
+             * admit.
+    }
+    + admit.
+    + admit.
+    + admit.
+    + admit.
+(*      destruct H7.
+      * destruct H7 as [? [? ?]].
+        subst. rewrite H32 in H12; inversion H12.
+        rewrite H32 in H22; inversion H22. subst.
+        clear H22 H12.
+        split. destruct H1. pose proof (mi_representable _ _ _ i H32).
+        destruct H1.
+        (* apply (mi_representable H32). *)
+        admit.
+        split; trivial.
+        split. admit.
+        split. clear -H1 H5. destruct H5 as [? [? ?]].
+        split; trivial. split. 
+        unfold Ptrofs.add; repeat rewrite Ptrofs.unsigned_repr_eq.
+        destruct H1.
+        repeat (split; try easy).
+      split; trivial.
+      (* Mem.address_inject. *)
+      (* Mem.valid_pointer_inject_no_overflow: *)
+      split; [admit|].
+      split; [rewrite H22 in H12; now inversion H12|].
+      split; [rewrite H22 in H12; inversion H12; subst;
+              unfold Ptrofs.add; rewrite <- H9; admit|].
+      split. 
+      intuition.
+      destruct H27.
+      * destruct H0 as [? [? ?]]. subst.
+        rewrite H12 in H22. inversion H22.
+        rewrite H12 in H32; inversion H32.
+        subst.
+        intuition; try easy.
+        5: { left. split; trivial; split; trivial.
+             unfold Ptrofs.add. split.
+             - repeat rewrite Ptrofs.unsigned_repr_eq.
+               admit.
+             - admit. }
+        admit. admit. admit. admit.
+      * destruct H0. destruct H0.
+        -- admit.
+        -- destruct H0. subst.
+           rewrite H12 in H22. inversion H22.
+           rewrite H12 in H32; inversion H32.
+           subst.
+           admit.
+           (* intuition; try easy. *)
+           (* 10 subgoals, none easy *) *)
+      (*
+(** External calls must commute with memory injections,
+  in the following sense. *)
+  ec_mem_inject:
+    forall ge1 ge2 vargs m1 t vres m2 f m1' vargs',
+    symbols_inject f ge1 ge2 ->
+    sem ge1 vargs m1 t vres m2 ->
+    Mem.inject f m1 m1' ->
+    Val.inject_list f vargs vargs' ->
+    exists f', exists vres', exists m2',
+       sem ge2 vargs' m1' t vres' m2'
+    /\ Val.inject f' vres vres'
+    /\ Mem.inject f' m2 m2'
+    /\ Mem.unchanged_on (loc_unmapped f) m1 m2
+    /\ Mem.unchanged_on (loc_out_of_reach f m1) m1' m2'
+    /\ inject_incr f f'
+    /\ inject_separated f f' m1 m1';
+       *)
+  - intros. destruct H as [_ [? _]]. subst t. simpl. omega.
+  - intros. generalize H. destruct H as [_ [? _]]. subst t1. inversion H0. subst t2. clear H0. intro H.
+      exists vres1, m1. apply H.
+  - intros. destruct H as [? [? ?]]. destruct H0 as [? [? ?]].
+      subst m1 m2 t1 t2. split. constructor. intros _.
+      split; trivial.
+      do 4 (destruct vargs; try destruct v; try contradiction).
+      destruct H2 as [_ [_ [_ [_ [_ [_ [_ ?]]]]]]].
+      destruct H4 as [_ [_ [_ [_ [_ [_ [_ ?]]]]]]].
+      intuition; congruence.
+Admitted.
